### 4.4.1

For each of the following grammars, devise predictive parsers
and show the parsing tables. You may left-factor and/or eliminate left-recursion
from your grammars î€Œrst.

---

#### a) $S \rightarrow 0 \ S \ 1 \ | \ 0 \ 1$
```
<S> ::= 0A
// <A> ::= S1 | 1 
<A> ::= 0A1 | 1
```
|   | 0      | 1    | $ | FIRST | FOLLOW |
|---|--------|------|---|-------|--------|
| S | ```S->0A```  |      |   | ```0```     | ```$```      |
| A | ```S->0A1``` | ```A->1``` |   | ```0```, ```1```  | ```$```, ```1```   |

#### b) $S \rightarrow +SS \ | \ *SS \ | \ a $

|   | a          | +            | *            | $ | FIRST                     | FOLLOW                             |
|---|------------|--------------|--------------|---|---------------------------|------------------------------------|
| S | ```S->a``` | ```S->+SS``` | ```S->*SS``` |   | ```+```, ```*```, ```a``` | '''$''', ```a```, ```+```, ```*``` |


#### c) $S \rightarrow S(S)S \ | \ \epsilon$ 

```EBNF
S = A
A = (S)SA | e
```
|   | (                          | )          | $          | FIRST         | FOLLOW                    |
|---|----------------------------|------------|------------|---------------|---------------------------|
| S | ```S->A```                 | ```S->A``` | ```S->A``` | (, $\epsilon$ | ```$```, ```(```, ```)``` |
| A | ```A->(S)SA```, ```A->e``` | ```A->e``` | ```A->e``` | (, $\epsilon$ | ```$```, ```(```, ```)``` |

#### d) $S \rightarrow S+S \ | \ SS \ | \ (S) \ | \ S* \ | \ a$
1. left factoring
```
S -> SA | (S) | a
A -> +S | S | *
```
2. eliminating left recursion
```
1. 
S -> aB | (S)B
B -> AB | e
A -> +S | S | *

2.
S -> aB | (S)B
B -> AB | e
A -> +S | aB | (S)B | *
```
|   | a                     | (                     | )             | +                    | *                    | $             | FIRST                  | FOLLOW           |
|---|-----------------------|-----------------------|---------------|----------------------|----------------------|---------------|------------------------|------------------|
| S | S->aB                 | S->(S)B               |               |                      |                      |               | a, (                   | a, +, *, (, ), $ |
| A | A->aB                 | A->(S)B               |               | A->+S                | A->*                 |               | a, +, *, (             | a, +, *, (, ), $ |
| B | B->AB,  B->$\epsilon$ | B->AB,  B->$\epsilon$ | B->$\epsilon$ | B->AB, B->$\epsilon$ | B->AB, B->$\epsilon$ | B->$\epsilon$ | a, +, *, (, $\epsilon$ | a, +, *, (, ), $ |


### 4.4.2
Is it possible to modify the grammar in Exercise 4.2.1 in some way to construct a predictive parser that corresponds to the language in this exercise (postfix expressions whose operands are a)?

---
$$S -> SS+ \ | \ SS* \ | \ a$$

1. It's not LL(1)

```
S -> SS+ | SS* | a

S -> aA 
A -> S+A | S*A | EPSILON

S -> aA
A -> aA+A | aA*A | EPSILON
```

2. Technique now
```
S -> S S O | a
O -> + | *

S -> a A 
A -> S O A | EPSILON  
O -> + | *

S -> a A
A -> a A O A| EPSILON
0 -> + | *
```
|   | a        | +               | *             | $               | FIRST         | FOLLOW     |
|---|----------|-----------------|---------------|-----------------|---------------|------------|
| S | S -> aA  |                 |               |                 | a             | $          |
| A | A -> aAO | A -> $\epsilon$ | A->$\epsilon$ | A -> $\epsilon$ | a, $\epsilon$ | +, *, $    |
| O |          | O -> +          | O -> *        |                 | +, *          | a, +, *, $ |


### 4.4.3
Compute FIRST and FOLLOW for the grammar of Exercise
4.2.1.

---


### 4.4.4
Compute FIRST and FOLLOW for each of the grammars of
Exercise 4.2.2.

---

check the 4.4.2 above.